Get rid of NEList usage and changed them to valuset-style.

src/AByteFile.v
@@ -26,7 +26,6 @@ Require Import GenSepAuto.
 Require Import DiskSet.
 Require Import BFile.
 Require Import Bytes.
-Require Import NEList.
 Require Import VBConv.
 
 Set Implicit Arguments.
@@ -188,25 +187,26 @@ else                                                   (* if read length is not 
   Ret ^(fms, nil)
 }.
 
-Definition write_first_block lxp ixp inum fms block_off byte_off data :=
- let^ (fms, first_block) <- BFILE.read lxp ixp inum block_off fms;   (* get first block *) 
-    let first_block_list := valu2list first_block in
-    let first_block_write := list2valu ((firstn byte_off first_block_list)     (* Construct first block*)
-                              ++data++(skipn (byte_off + length data) first_block_list))%list in 
+Definition write_to_block lxp ixp inum fms block_off byte_off data :=
+ let^ (fms, block) <- BFILE.read lxp ixp inum block_off fms;   (* get first block *) 
+    let block_list := valu2list block in
+    let block_write := list2valu ((firstn byte_off block_list)     (* Construct first block*)
+                              ++data++(skipn (byte_off + length data) block_list))%list in 
     (*Write first block*)                          
+    let '(al, ms) := (BFILE.MSAlloc fms, BFILE.MSLL fms) in
     let^ (ms, bn) <-INODE.getbnum lxp ixp inum block_off (BFILE.MSLL fms);
-    ms <- LOG.write lxp (# bn) first_block_write ms;
-Ret (fms).
+    ms <- LOG.write lxp (# bn) block_write ms;
+Ret (BFILE.mk_memstate al ms).
 
 
 
 
-Definition write_middle_blocks lxp ixp inum fms block_off num_of_full_blocks data:=
+Definition write_middle_blocks lxp ixp inum fms block_off first_write_length num_of_full_blocks data:=
      let block_size := valubytes in
     let^ (temp) <- (ForN_ (fun i => (pair_args_helper (fun d (_:unit) =>
-      
-      fms <- write_first_block lxp ixp inum fms (block_off + i) 0 
-                (get_sublist data (i*block_size) block_size);
+
+      let^ (ms, bn) <- INODE.getbnum lxp ixp inum (block_off+i) (BFILE.MSLL fms);(* get i'th block number *)
+      ms <- LOG.write lxp (# bn) (list2valu (get_sublist data (first_write_length + i*block_size) block_size)) ms;
       Ret ^(nil: list byte)
       
       ))) 0 num_of_full_blocks
@@ -226,8 +226,14 @@ Definition write_middle_blocks lxp ixp inum fms block_off num_of_full_blocks dat
             Rof ^((nil:list byte));
 Ret ^(nil: list byte). *)
  
-Definition write_last_block lxp ixp inum fms block_off data:=
-    fms <- write_first_block lxp ixp inum fms block_off 0 data;
+Definition write_last_block lxp ixp inum fms off_final len_final data:=
+    let block_size := valubytes in 
+    let^ (fms, last_block) <- BFILE.read lxp ixp inum off_final fms;   (* get final block *)
+    let last_block_write := list2valu ((get_sublist data off_final len_final) 
+                            ++ (get_sublist (valu2list last_block) len_final (block_size - len_final)))%list in
+                            
+    let^ (ms, bn) <- INODE.getbnum lxp ixp inum (off_final) (BFILE.MSLL fms);(* get final block number *)
+    ms <- LOG.write lxp (# bn) last_block_write ms;
     Ret (fms).
 
 Definition write lxp ixp inum off data fms :=
@@ -238,20 +244,19 @@ Definition write lxp ixp inum off data fms :=
     let byte_off := off mod block_size in          (* calculate byte offset *)
     let first_write_length := min (block_size - byte_off) len in (*# of bytes that will be read from first block*)
     
-    fms <- write_first_block lxp ixp inum fms block_off byte_off (firstn first_write_length data);
+    fms <- write_to_block lxp ixp inum fms block_off byte_off (firstn first_write_length data);
     
     let block_off := S block_off in
     let len_remain := (len - first_write_length) in  (* length of remaining part *)
-    let data_remain := skipn first_write_length data in
     let num_of_full_blocks := (len_remain / block_size) in (* number of full blocks in length *)
     
-   fms <- write_middle_blocks lxp ixp inum fms block_off num_of_full_blocks data_remain;
+   fms <- write_middle_blocks lxp ixp inum fms block_off first_write_length num_of_full_blocks data;
     
     let off_final := (block_off + num_of_full_blocks) in (* offset of final block *)
     let len_final := (len_remain - num_of_full_blocks * block_size) in (* final remaining length *)
-    let data_final := skipn (num_of_full_blocks * block_size) data_remain in
+    
     (*Write last block*)
-    fms <- write_last_block lxp ixp inum fms off_final data_final;
+    fms <- write_last_block lxp ixp inum fms off_final len_final data;
   
     Ret (fms).
     
@@ -300,7 +305,7 @@ Qed.
 
 Lemma pick_from_block: forall F f block_off vs i def def', 
 i < valubytes -> (F * block_off |-> vs)%pred (list2nmem (BFILE.BFData f)) ->
-selN (valu2list (latest vs)) i def = selN (valu2list (latest (selN (BFILE.BFData f) block_off def'))) i def.
+selN (valu2list (fst vs)) i def = selN (valu2list (fst (selN (BFILE.BFData f) block_off def'))) i def.
 Proof.
 intros.
 erewrite block_content_match with (f:=f) (vs:=vs) (block_off:= block_off) (def:= def').
@@ -551,7 +556,7 @@ repeat destruct H0.
 apply valuset2bytesets_len.
 Qed.
 
-(* Fact content_match: forall Fd f pfy ufy fy i j data,
+Fact content_match: forall Fd f pfy ufy fy i j data,
 proto_bytefile_valid f pfy ->
 unified_bytefile_valid pfy ufy ->
 bytefile_valid ufy fy ->
@@ -559,8 +564,8 @@ bytefile_valid ufy fy ->
 j < valubytes ->
 length data > 0 ->
 j + length data <= valubytes ->
-get_sublist (valu2list (latest (bytesets2valuset
-(get_sublist (UByFData ufy) (i * valubytes) valubytes)))) j (length data) = map (@latest byte) data.
+get_sublist (valu2list (fst (bytesets2valuset
+(get_sublist (UByFData ufy) (i * valubytes) valubytes)))) j (length data) = map fst data.
  Proof.
  intros.
        
@@ -575,80 +580,33 @@ rewrite H1'.
 rewrite firstn_length.
 rewrite skipn_length.
 rewrite Min.min_l.
-rewrite <- firstn_map_comm.
-rewrite Nat.add_comm.
-rewrite <- skipn_skipn with (m:= i * valubytes).
 rewrite H0.
 rewrite concat_hom_skipn.
-
-
 replace (firstn valubytes (concat (skipn i (PByFData pfy))))
   with (firstn (1 * valubytes) (concat (skipn i (PByFData pfy)))).
 rewrite concat_hom_firstn.
 rewrite firstn1.
 rewrite skipn_selN.
-rewrite <- skipn_map_comm.
-rewrite concat_map.
-repeat rewrite <- skipn_firstn_comm.
-rewrite concat_hom_O with (k:= valubytes).
-repeat erewrite selN_map.
-rewrite skipn_selN.
+rewrite <- firstn_map_comm.
 rewrite <- plus_n_O.
-unfold bytesets2valuset.
-
-
-Fact latest_l2n: forall A (l: list A) def def',
-l <> nil -> latest (list2nelist def l) = selN l 0 def'.
-Proof.
-intros.
-unfold list2nelist.
-destruct l.
-destruct H; reflexivity.
-simpl.
-unfold singular.
-rewrite pushdlist_app; rewrite app_nil_r.
-rewrite rev_involutive.
-rewrite <-minus_n_O.
-destruct (length l); reflexivity.
-Qed.
-
-erewrite latest_l2n.
-unfold nelist2list.
-Fact b2v_rec_selN: forall i j l def def',
-i > 0 -> length l = i -> j < i ->
-selN (bytesets2valuset_rec l i) j def = map (selN' j def') l.
-simpl.
-
-unfold list2nelist.
-simpl.
+rewrite Nat.add_comm.
+rewrite <- skipn_skipn with (m:= i * valubytes).
+rewrite concat_hom_skipn.
+rewrite <- skipn_map_comm.
+rewrite H.
+rewrite concat_map.
+erewrite selN_map.
 rewrite valuset2bytesets2valuset.
 
 repeat rewrite skipn_map_comm.
 repeat rewrite <- skipn_firstn_comm.
-About concat_hom_O.
 rewrite concat_hom_O with (k:= valubytes).
-erewrite selN_map.
-rewrite selN_map with (default':=valuset0).
-rewrite skipn_selN.
+repeat erewrite selN_map.
+erewrite skipn_selN.
 rewrite <- plus_n_O.
 unfold valuset2bytesets.
-rewrite maplatest_v2b.
-erewrite selN_map.
-(selN (BFILE.BFData f) i valuset0).
-simpl.
-unfold nelist2list.
-unfold latest.
-remember (snd (selN (BFILE.BFData f) i valuset0)) as s.
-
-rewrite selN_app1.
-unfold latest; simpl.
-destruct (selN (BFILE.BFData f) i valuset0).
-
-unfold valu2list.
-simpl.
-unfold bsplit1_dep, bsplit2_dep; simpl.
-rewrite skipn_map_comm.
-rewrite maplatest_v2b.
+unfold byteset2list.
+rewrite map_cons.
 rewrite mapfst_valuset2bytesets.
 reflexivity.
 
@@ -703,7 +661,7 @@ apply byteset0.
 Grab Existential Variables.
 apply nil.
 apply valuset0.
-Qed. *)
+Qed.
 
 
 
@@ -727,47 +685,94 @@ rewrite listmatch_length_pimpl in H0.
 sepauto.
 Qed.
 
-
-
-
-Fact fst_l2nel: forall A (l:list A) def,
-fst(list2nelist def l) = selN l (length l -1) def.
-Proof.
-intros.
-induction l.
-reflexivity.
-simpl.
-rewrite <- minus_n_O.
-unfold singular; rewrite pushdlist_app.
-simpl.
-reflexivity.
-Qed.
-
-
-
-
-Fact nel2l_O: forall A (l: nelist A) def,
-selN (nelist2list l) 0 def = latest l.
-Proof.
-intros.
-induction l.
-unfold nelist2list, latest.
-simpl.
-destruct b; reflexivity.
-Qed.
-
-
-
 (*Specs*)
 
 
+Theorem read_first_block_ok: forall lxp bxp ixp inum fms block_off byte_off read_length,
+ {< F Fm Fi Fd m0 m flist ilist frees f fy (data: list byteset),
+    PRE:hm
+          let file_length := (# (INODE.ABytes (ByFAttr fy))) in
+          let block_size := valubytes in
+           rep lxp bxp ixp flist ilist frees inum  F Fm Fi fms m0 m hm f fy  *
+           [[[ (ByFData fy) ::: (Fd * (arrayN (ptsto (V:= byteset)) (block_off * block_size + byte_off) data)) ]]] *
+           [[ 0 < read_length]] * 
+           [[ length data = read_length ]] *
+           [[ byte_off + read_length <= block_size]]
+    POST:hm' RET:^(fms', r)
+          LOG.rep lxp F (LOG.ActiveTxn m0 m) (BFILE.MSLL fms') hm' *
+          [[ r = (map fst data) ]] *
+          [[BFILE.MSAlloc fms = BFILE.MSAlloc fms' ]]
+    CRASH:hm'  exists (fms':BFILE.memstate),
+           LOG.rep lxp F (LOG.ActiveTxn m0 m) (BFILE.MSLL fms') hm'
+    >} read_first_block lxp ixp inum fms block_off byte_off read_length.
+Proof.
+unfold read_first_block, rep.
+prestep.
+norm.
+unfold stars; cancel.
+intuition; eauto.
+
+eapply inlen_bfile; eauto.
+omega.
+
+eapply protobyte2block; eauto.
+eapply unifiedbyte2protobyte 
+  with (a:= block_off * valubytes + byte_off) (k:= valubytes) in H11; try omega.
+rewrite div_eq in H11; try omega.
+apply H11.
+
+eapply proto_len; eauto.
+eapply byte2unifiedbyte; eauto.
+pred_apply.
+rewrite arrayN_isolate with (i:=0).
+rewrite <- plus_n_O .
+cancel.
+auto.
+
+step.
+
+eapply content_match; eauto.
+omega.
+Grab Existential Variables.
+apply byteset0. 
+Qed.
 
 
 
 
+Theorem read_middle_blocks_ok: forall lxp bxp ixp inum fms block_off num_of_full_blocks,
+ {< F Fm Fi Fd m0 m flist ilist frees f fy (data: list byteset),
+    PRE:hm
+          let file_length := (# (INODE.ABytes (ByFAttr fy))) in
+          let block_size := valubytes in
+           rep lxp bxp ixp flist ilist frees inum  F Fm Fi fms m0 m hm f fy *
+           [[[ (ByFData fy) ::: (Fd * (arrayN (ptsto (V:=byteset)) (block_off * block_size) data))]]] *
+           [[ num_of_full_blocks > 0 ]] *
+           [[ length data = mult num_of_full_blocks block_size ]]
+    POST:hm' RET:^(fms', r)
+          LOG.rep lxp F (LOG.ActiveTxn m0 m) (BFILE.MSLL fms') hm' *
+          [[ r = (map fst data)]] *
+          [[BFILE.MSAlloc fms = BFILE.MSAlloc fms' ]]
+    CRASH:hm'  exists (fms':BFILE.memstate),
+           LOG.rep lxp F (LOG.ActiveTxn m0 m) (BFILE.MSLL fms') hm'
+    >} read_middle_blocks lxp ixp inum fms block_off num_of_full_blocks.
+Proof.
+unfold read_middle_blocks.
+prestep.
+norm.
+unfold stars; cancel.
+unfold rep; cancel.
+intuition; eauto.
+rewrite valubytes_is; reflexivity.
+eapply pimpl_ok2.
+monad_simpl.
+apply read_first_block_ok.
+Admitted.
 
 
-(* Theorem read_last_block_ok: forall lxp bxp ixp inum fms block_off read_length,
+(* 
+
+Theorem read_last_block_ok: forall lxp bxp ixp inum fms block_off read_length,
  {< F Fm Fi Fd m0 m flist ilist frees f fy data,
     PRE:hm
           let file_length := (# (INODE.ABytes (ByFAttr fy))) in
@@ -779,7 +784,7 @@ Qed.
            [[ read_length < block_size]]
     POST:hm' RET:^(fms', r)
           LOG.rep lxp F (LOG.ActiveTxn m0 m) (BFILE.MSLL fms') hm' *
-          [[ r = map (@latest byte) data ]] *
+          [[ r = map fst data ]] *
           [[BFILE.MSAlloc fms = BFILE.MSAlloc fms' ]]
     CRASH:hm'  exists (fms':BFILE.memstate),
            LOG.rep lxp F (LOG.ActiveTxn m0 m) (BFILE.MSLL fms') hm'
@@ -829,310 +834,6 @@ Grab Existential Variables.
 apply byteset0.
 Qed.
 
- *)
-
-Theorem read_first_block_ok: forall lxp bxp ixp inum fms block_off byte_off read_length,
- {< F Fm Fi Fd m0 m flist ilist frees f fy (data: list byteset),
-    PRE:hm
-          let file_length := (# (INODE.ABytes (ByFAttr fy))) in
-          let block_size := valubytes in
-           rep lxp bxp ixp flist ilist frees inum  F Fm Fi fms m0 m hm f fy  *
-           [[[ (ByFData fy) ::: (Fd * (arrayN (ptsto (V:= byteset)) (block_off * block_size + byte_off) data)) ]]] *
-           [[ 0 < read_length]] * 
-           [[ length data = read_length ]] *
-           [[ byte_off + read_length <= block_size]]
-    POST:hm' RET:^(fms', r)
-          LOG.rep lxp F (LOG.ActiveTxn m0 m) (BFILE.MSLL fms') hm' *
-          [[ r = (map (@latest byte) data) ]] *
-          [[BFILE.MSAlloc fms = BFILE.MSAlloc fms' ]]
-    CRASH:hm'  exists (fms':BFILE.memstate),
-           LOG.rep lxp F (LOG.ActiveTxn m0 m) (BFILE.MSLL fms') hm'
-    >} read_first_block lxp ixp inum fms block_off byte_off read_length.
-Proof.
-unfold read_first_block, rep.
-step.
-
-eapply inlen_bfile; eauto.
-omega.
-
-eapply protobyte2block; eauto.
-eapply unifiedbyte2protobyte with (a:= block_off * valubytes + byte_off) (k:= valubytes) in H11; try omega.
-rewrite div_eq in H11; try omega.
-apply H11.
-
-eapply proto_len; eauto.
-eapply byte2unifiedbyte; eauto.
-pred_apply.
-rewrite arrayN_isolate with (i:=0).
-rewrite <- plus_n_O .
-cancel.
-auto.
-
-step.
-
-apply arrayN_list2nmem in H8 as H1'.
-rewrite H10 in H1'.
-rewrite <- skipn_firstn_comm in H1'.
-rewrite firstn_firstn in H1'.
-rewrite Min.min_l in H1'.
-rewrite skipn_firstn_comm in H1'.
-rewrite H1'.
-unfold get_sublist.
-rewrite firstn_length.
-rewrite skipn_length.
-rewrite Min.min_l.
-rewrite <- firstn_map_comm.
-rewrite Nat.add_comm.
-rewrite <- skipn_skipn with (m:= block_off * valubytes).
-rewrite H11.
-rewrite concat_hom_skipn.
-
-
-replace (firstn valubytes (concat (skipn block_off (PByFData pfy))))
-  with (firstn (1 * valubytes) (concat (skipn block_off (PByFData pfy)))).
-rewrite concat_hom_firstn.
-rewrite firstn1.
-rewrite skipn_selN.
-rewrite <- skipn_map_comm.
-rewrite concat_map.
-repeat rewrite <- skipn_firstn_comm.
-rewrite concat_hom_O with (k:= valubytes).
-rewrite selN_map with (default':=nil).
-rewrite skipn_selN.
-rewrite <- plus_n_O.
-
-rewrite H12.
-rewrite selN_map with (default':= valuset0).
-rewrite valuset2bytesets2valuset.
-
-
-
-eapply protobyte2block with (a:= block_off) in H12.
-eapply list2nmem_sel in H12.
-rewrite <- H12.
-
-rewrite bytesets2valuset2bytesets.
-
-unfold bytesets2valuset.
-rewrite fst_l2nel.
-rewrite nel2l_O.
-unfold nelist2list.
-simpl.
-rewrite app_length.
-simpl.
-rewrite map_app.
-simpl.
-
-Fact b2v_rec_length: forall i l,
-i <= length l ->
-length (bytesets2valuset_rec l i) = i.
-Proof.
-induction i; intros.
-reflexivity.
-destruct l.
-inversion H.
-simpl.
-rewrite IHi.
-reflexivity.
-destruct l.
-simpl in H.
-
-
-
-Fact b2v_rec_expand: forall l i,
-i > 0 -> l<> nil ->
-bytesets2valuset_rec l i =  (list2valu (map (selN' 0 byte0) l) )::(bytesets2valuset_rec (map (skipn 1) l) (i-1)).
-Proof.
-intros.
-induction i.
-inversion H.
-
-simpl.
-rewrite <- minus_n_O.
-destruct l.
-destruct H0; reflexivity.
-reflexivity.
-Qed.
-
-simpl.
-rewrite map_length.
-omega.
-simpl in *.
-rewrite map_length; omega.
-Qed.
-
-rewrite b2v_rec_length.
-Search plus minus.
-replace (1 - 1) with 0 by omega.
-simpl.
-
-
-
-reflexivity.
-simpl.
-destruct a.
-simpl.
-
-
-
-destruct (?b).
-unfold nelist2list.
-rewrite map_app.
-simpl.
-rewrite maplatest_v2b.
-
-
-unfold bytesets2valuset.
-simpl.
-
-
-
-simpl.
-rewrite app_length,
-simpl.
-unfold selN. 
-
-
-
-remember (selN (BFILE.BFData f) block_off valuset0) as s.
-destruct s.
-pose proof H10.
-eapply byte2unifiedbyte with (a:= block_off * valubytes + 0) in H10.
-eapply unifiedbyte2protobyte with (k:= valubytes)(pfy:=pfy) in H10.
-rewrite div_eq in H10.
-eapply list2nmem_sel in H10.
-rewrite <- Heqs in H10.
-apply length_zero_iff_nil in H10.
-unfold get_sublist in H10.
-rewrite firstn_length in H10.
-rewrite skipn_length in H10.
-
-
-Fact min_O: forall n m,
-Init.Nat.min n m = 0 -> n = 0 \/ m = 0.
-intros.
-destruct n.
-left; reflexivity.
-right.
-destruct m.
-reflexivity.
-inversion H.
-Qed.
-
-
-
-apply min_O in H10.
-destruct H10.
-rewrite valubytes_is in H6; inversion H6.
-Search minus 0.
-apply list2nmem_arrayN_bound in H8.
-destruct H8.
-rewrite H8 in H7; inversion H7.
-rewrite H4 in H8.
-rewrite firstn_length in H8.
-apply Min.min_glb_r in H8.
-About le2lt_l.
-apply le2lt_l in H8.
-apply lt_weaken_l in H8.
-Search minus 0.
-apply Nat.sub_gt in H8.
-apply H8 in H6; inversion H6.
-omega.
-rewrite valubytes_is; omega.
-auto.
-eapply proto_len; eauto.
-rewrite valubytes_is; omega.
-rewrite <- plus_n_O.
-eapply list2nmem_ptsto_cancel.
-apply list2nmem_arrayN_bound in H8.
-destruct H8.
-rewrite H6 in H7; inversion H7.
-apply le2lt_l in H6.
-apply lt_weaken_l in H6.
-apply H6.
-omega.
-
-simpl.
-unfold bytesets2valuset.
-simpl.
-
-unfold valu2list.
-rewrite b2v_rec_selN.
-
-rewrite H4.
-Search list2nmem ptsto.
-rewrite H11.
-Search list2nmem lt ptsto.
-eapply byte2unifiedbyte in H4.
-apply Nat.le_add_le_sub_l.
-Search le plus.
-rewrite <- Heqs in H4.
-simpl.
-unfold valu2list.
-simpl.
-unfold bytesets2valuset.
-unfold bytesets2valuset_rec.
-
-simpl.
-unfold list2nelist; simpl.
-
-
-Fact latest_l2n: forall A (l: list A) def def',
-l <> nil -> latest (list2nelist def l) = selN l 0 def'.
-Proof.
-intros.
-unfold list2nelist.
-destruct l.
-destruct H; reflexivity.
-simpl.
-unfold singular.
-rewrite pushdlist_app; rewrite app_nil_r.
-rewrite rev_involutive.
-rewrite <-minus_n_O.
-destruct (length l); reflexivity.
-Qed.
-
-
-eapply content_match; eauto.
-omega.
-Grab Existential Variables.
-apply byteset0. 
-Qed.
-
-
-Theorem read_middle_blocks_ok: forall lxp bxp ixp inum fms block_off num_of_full_blocks,
- {< F Fm Fi Fd m0 m flist ilist frees f fy (data: list byteset),
-    PRE:hm
-          let file_length := (# (INODE.ABytes (ByFAttr fy))) in
-          let block_size := valubytes in
-           rep lxp bxp ixp flist ilist frees inum  F Fm Fi fms m0 m hm f fy *
-           [[[ (ByFData fy) ::: (Fd * (arrayN (ptsto (V:=byteset)) (block_off * block_size) data))]]] *
-           [[ num_of_full_blocks > 0 ]] *
-           [[ length data = mult num_of_full_blocks block_size ]]
-    POST:hm' RET:^(fms', r)
-          LOG.rep lxp F (LOG.ActiveTxn m0 m) (BFILE.MSLL fms') hm' *
-          [[ r = (map (@latest byte) data)]] *
-          [[BFILE.MSAlloc fms = BFILE.MSAlloc fms' ]]
-    CRASH:hm'  exists (fms':BFILE.memstate),
-           LOG.rep lxp F (LOG.ActiveTxn m0 m) (BFILE.MSLL fms') hm'
-    >} read_middle_blocks lxp ixp inum fms block_off num_of_full_blocks.
-Proof.
-unfold read_middle_blocks, rep; step.
-rewrite valubytes_is; reflexivity.
-prestep.
-norm.
-unfold stars.
-simpl.
-rewrite LOG.rep_hashmap_subset by eauto.
-cancel.
-intuition.
-eapply pimpl_pre2; intros.
-repeat ( apply sep_star_lift_l; intros ).
-unfold pimpl, lift; intros.
-eapply pimpl_ok2. repeat monad_simpl.
-Focus 2. intros.
-apply pimpl_refl.
-Admitted.
 
 Theorem read_ok : forall lxp bxp ixp inum off len fms,
     {< F Fm Fi Fd m0 m flist ilist frees f fy data,
@@ -1144,7 +845,7 @@ Theorem read_ok : forall lxp bxp ixp inum off len fms,
            [[ length data = len ]]
     POST:hm' RET:^(fms', r)
           LOG.rep lxp F (LOG.ActiveTxn m0 m) (BFILE.MSLL fms') hm' *
-          [[ r = map (@latest byte) data]] *
+          [[ r = map fst data]] *
           [[BFILE.MSAlloc fms = BFILE.MSAlloc fms' ]]
     CRASH:hm'  exists (fms':BFILE.memstate),
            LOG.rep lxp F (LOG.ActiveTxn m0 m) (BFILE.MSLL fms') hm'
@@ -1165,12 +866,14 @@ destruct (lt_dec 0 (Init.Nat.min (length data) (a0 - off) -
           (Init.Nat.min (length data) (a0 - off))) / valubytes * valubytes)).
           constructor.
 destruct_lift H.
-Admitted.
+Admitted. *)
 
-Fixpoint updN_list A (l: list A) off (l1: list A): list A :=
+Definition upd_byteset bs b: byteset := (b, (fst bs)::(snd bs)).
+
+Fixpoint updN_list (l: list byteset) off (l1: list byte): list byteset :=
 match l1 with
 | nil => l
-| h::t => updN_list (updN l off h) (S off) t
+| h::t => updN_list ((firstn off l)++((upd_byteset (selN l off byteset0) h)::(skipn (S off) l))) (S off) t
 end.
 
 Theorem write_first_block_ok : forall lxp bxp ixp inum block_off byte_off data fms,
@@ -1183,17 +886,19 @@ Theorem write_first_block_ok : forall lxp bxp ixp inum block_off byte_off data f
            [[ byte_off + length data <= valubytes ]] 
     POST:hm' RET:fms'  exists m' flist' f' fy',
            rep lxp bxp ixp flist' ilist frees inum  F Fm Fi fms' m0 m' hm' f' fy' *
-           [[[ (ByFData fy') ::: (Fd * arrayN (ptsto (V:=byteset)) (block_off * valubytes + byte_off) 
-            (map (@singular byte) data))]]] *
-           [[ fy' = mk_bytefile (updN_list (ByFData fy) (block_off * valubytes + byte_off) 
-           (map (@singular byte) data)) (ByFAttr fy) ]] *
+           [[[ (ByFData fy') ::: (Fd * arrayN (ptsto (V:=byteset)) 
+           (block_off * valubytes + byte_off) (updN_list old_data 0 data))]]] *
+           [[ fy' = mk_bytefile (updN_list (ByFData fy) (block_off * valubytes + byte_off) data) (ByFAttr fy)  ]] *
            [[ BFILE.MSAlloc fms = BFILE.MSAlloc fms' ]]
     CRASH:hm'  LOG.intact lxp F m0 hm'
-    >} write_first_block lxp ixp inum fms block_off byte_off data.
+    >} write_to_block lxp ixp inum fms block_off byte_off data.
 
 Proof.
-unfold write_first_block, rep.
-step.
+unfold write_to_block, rep.
+prestep.
+norm.
+unfold stars; cancel.
+intuition; eauto.
 
 eapply inlen_bfile; try eauto; try omega.
 
@@ -1223,7 +928,7 @@ rewrite valubytes_is in *; omega.
 omega.
 
 Show Existentials.
-Existential  9:= ilist.
+Existential  10:= ilist.
 auto.
 apply list2nmem_inbound in H13.
 unfold BFILE.rep in H0.
@@ -1247,7 +952,7 @@ apply H21.
 
 step.
 
-pose proof H0 as H0'.
+(* pose proof H0 as H0'.
 unfold BFILE.rep in H0.
 destruct_lift H0.
 unfold BFILE.file_match in H0.
@@ -1285,54 +990,7 @@ eapply list2nmem_sel with (F:= (F'
               erewrite selN_map in H0.
 rewrite H14 in H0.
 eapply list2nmem_sel in H13.
-rewrite <- H13 in H0.
-3: apply H20.
-Focus 2.
-eapply list2nmem_sel in H13 as H13'.
-erewrite iblocks_file_len_eq with (flist:= flist).
-eapply inlen_bfile; eauto; try omega.
-rewrite <- H13'; eauto.
-
-
-apply list2nmem_inbound in H13.
-unfold BFILE.rep in H0'.
-replace (length ilist) with (length flist).
-apply H13.
-rewrite listmatch_length_pimpl in H0'.
-destruct_lift H0'.
-eauto.
-eauto.
-
-Focus 2.
-rewrite combine_length.
-rewrite map_length.
-eapply list2nmem_sel in H13 as H13'.
-erewrite iblocks_file_len_eq with (flist:=flist).
-repeat rewrite <- H13'.
-rewrite Nat.min_id.
-eapply inlen_bfile; eauto; try omega.
-apply list2nmem_inbound in H13.
-unfold BFILE.rep in H0'.
-replace (length ilist) with (length flist).
-apply H13.
-rewrite listmatch_length_pimpl in H0'.
-destruct_lift H0'.
-eauto.
-eauto.
-
-Focus 2.
-apply list2nmem_inbound in H13.
-apply H13.
-
-Focus 2.
-apply list2nmem_inbound in H13.
-unfold BFILE.rep in H0'.
-replace (length ilist) with (length flist).
-apply H13.
-rewrite listmatch_length_pimpl in H0'.
-destruct_lift H0'.
-eauto.
-eauto.
+rewrite <- H13 in H0. *)
 
 Focus 2.
 unfold pimpl; intros.
@@ -1357,10 +1015,11 @@ apply sep_star_comm in H14.
 apply ptsto_mem_except in H14.
 apply H14.
 
+eapply list2nmem_sel in H13 as H13'.
 erewrite iblocks_file_len_eq with (flist:= flist).
-eapply list2nmem_sel in H13.
-rewrite <- H13.
 eapply inlen_bfile; eauto; try omega.
+rewrite <- H13'; eauto.
+
 
 apply list2nmem_inbound in H13.
 unfold BFILE.rep in H0.
@@ -1404,19 +1063,76 @@ eauto.
 
 Focus 2.
 step.
-unfold pimpl; intros.
-eauto.
-unfold BFILE.rep in H0.
-sepauto.
-eapply pimpl_pre3 in H2.
-destruct H2.
-eauto.
-repeat destruct H2.
-repeat eexists.
-eauto.
-destruct_lift H14.
-rewrite H20.
 
+unfold BFILE.rep.
+cancel.
+unfold BFILE.file_match.
+cancel.
+unfold pimpl; intros.
+eapply listmatch_isolate with (i:= inum).
+
+apply list2nmem_inbound in H13.
+apply H13.
+
+
+apply list2nmem_inbound in H13.
+unfold BFILE.rep in H0.
+replace (length ilist) with (length flist).
+apply H13.
+rewrite listmatch_length_pimpl in H0.
+destruct_lift H0.
+eauto.
+pred_apply.
+cancel.
+
+unfold pimpl; intros.
+eapply listmatch_isolate with (i:= block_off).
+
+eapply list2nmem_sel in H13.
+rewrite <- H13.
+eapply inlen_bfile; eauto; try omega.
+
+rewrite map_length.
+erewrite iblocks_file_len_eq with (flist:= flist).
+eapply list2nmem_sel in H13.
+rewrite <- H13.
+eapply inlen_bfile; eauto; try omega.
+
+apply list2nmem_inbound in H13.
+unfold BFILE.rep in H0.
+replace (length ilist) with (length flist).
+apply H13.
+rewrite listmatch_length_pimpl in H0.
+destruct_lift H0.
+eauto.
+eauto.
+(* 
+assert(AS:(list2valu
+                (firstn byte_off
+                   (valu2list
+                      (fst
+                         (bytesets2valuset
+                            (get_sublist (UByFData ufy) (block_off * valubytes) valubytes)))) ++
+                 data ++
+                 skipn (byte_off + length data)
+                   (valu2list
+                      (fst
+                         (bytesets2valuset
+                            (get_sublist (UByFData ufy) (block_off * valubytes) valubytes))))),
+             nil) =  selN (BFILE.BFData (selN flist inum BFILE.bfile0)) block_off valuset0).
+Focus 1.           
+rewrite H11.  
+rewrite H12.
+unfold get_sublist.
+rewrite concat_hom_skipn.
+rewrite skipn_map_comm.
+replace valubytes with (1*valubytes) by omega.
+rewrite concat_hom_firstn.
+rewrite firstn1.
+erewrite selN_map.
+rewrite valuset2bytesets2valuset.
+rewrite skipn_selN.
+rewrite <- plus_n_O. *)
 Admitted.
 
 
