src/VBConv.v
@@ -6,18 +6,45 @@ Require Import FunctionalExtensionality.
 Require Import NArith.
 Require Import AsyncDisk.
 Require Import Bytes.
-Require Import NEList.
 
-Notation "'byteset'" := (nelist byte).
+Notation "'byteset'" := (byte * list byte)%type.
+
+
+Definition list2byteset {A} def (l: list A) : (A * list A) :=
+  match l with
+  | nil => (def, nil)
+  | h::t => (h,t)
+  end.
+
+Definition byteset2list {A} (nel: A * list A) : list A := (fst nel)::(snd nel).
+
+Lemma byteset2list2byteset: forall A (l: A * list A) def, 
+  list2byteset def (byteset2list l) = l.
+Proof.
+  intros.
+  unfold list2byteset, byteset2list.
+  symmetry; apply surjective_pairing.
+Qed.
+
+Lemma list2byteset2list: forall A (l: list A) def, 
+  l<>nil -> byteset2list (list2byteset def l) = l.
+Proof.
+  intros.
+  unfold list2byteset, byteset2list. 
+  destruct l.
+  destruct H; reflexivity.
+  reflexivity.
+Qed.
+
 
 Definition valu2bytes (v : valu) : bytes (1 + (valubytes - 1)).
   refine (@word2bytes valulen (1 + (valubytes - 1)) _ v).
   rewrite valulen_is. rewrite valubytes_is. reflexivity.
 Defined.
 
-Definition byteset0 := singular byte0.
+Definition byteset0 := (byte0, nil: list byte).
 Definition valu0 := bytes2valu  (natToWord (valubytes*8) 0).
-Definition valuset0 := singular valu0.
+Definition valuset0 := (valu0, nil: list valu).
 
 (* make this right padded *)
 Definition bytes2valubytes {sz} (b: bytes sz) : bytes valubytes :=
@@ -29,17 +56,11 @@ bytes2valu (bytes2valubytes (bcombine_list l)).
 Definition valu2list v : list byte :=
 bsplit_list (valu2bytes v).
 
-Fixpoint make_all_list {A: Type} (l: list A): list (list A):=
+(* Fixpoint make_all_list {A: Type} (l: list A): list (list A):=
 match l with
 | nil => nil
 | h::t => (cons h nil)::(make_all_list t)
-end.
-
-Fixpoint maxlist l: nat :=
-match l with
-| nil => 0
-| h::t => max h (maxlist t)
-end.
+end. *)
 
 Definition selN' {A: Type} i def (l: list A): A :=
 selN l i def.
@@ -50,12 +71,12 @@ match i with
 | O => nil
 | S i' => match vs with
     | nil => nil
-    | _ =>  (list2nelist byte0 (map (selN' 0 byte0) vs))::(valuset2bytesets_rec (map (skipn 1) vs) i')
+    | _ =>  (list2byteset byte0 (map (selN' 0 byte0) vs))::(valuset2bytesets_rec (map (skipn 1) vs) i')
     end
 end.
 
 Definition valuset2bytesets (vs: valuset): list byteset :=
-valuset2bytesets_rec (map valu2list (nelist2list vs)) valubytes.
+valuset2bytesets_rec (map valu2list (byteset2list vs)) valubytes.
 
 Fixpoint bytesets2valuset_rec (bs: list (list byte) ) i: list valu :=
 match i with
@@ -67,20 +88,14 @@ match i with
 end.
 
 Definition bytesets2valuset (bs: list byteset) : valuset :=
-list2nelist valu0 (bytesets2valuset_rec (map (@nelist2list byte) bs) (length(nelist2list(selN bs 0 byteset0)))).
+list2byteset valu0 (bytesets2valuset_rec (map (@byteset2list byte) bs) (length(byteset2list(selN bs 0 byteset0)))).
 
 Definition get_sublist {A:Type}(l: list A) (off len: nat) : list A :=
 firstn len (skipn off l).
+
   
 (* Lemmas *)
 
-Lemma make_all_list_len: forall (A:Type) (l: list A),
- length(make_all_list l) = length l.
-Proof.
-induction l.
-reflexivity.
-simpl; rewrite IHl; reflexivity.
-Qed.
 
 Lemma valu2list_len : forall v,
  length(valu2list v) = valubytes.
@@ -92,46 +107,15 @@ rewrite valubytes_is.
 reflexivity.
 Qed.
 
-(* Lemma maxlist_len: forall l, 
-l <> nil -> 
-maxlist (map (fun x : valu => length (valu2list x)) l) = valubytes.
-Proof.
-induction l; intros.
-destruct H; reflexivity.
-simpl.
-rewrite valu2list_len.
-destruct l.
-simpl.
-apply Nat.max_0_r.
-rewrite IHl.
-apply Nat.max_id.
-unfold not.
-intros; inversion H0.
-Qed. *)
-
-
-Lemma valuset2bytesets_rec_expand: forall l i a,
+Lemma valuset2bytesets_rec_expand: forall i a l,
    i > 0 ->
   valuset2bytesets_rec (a::l) i = 
-  (list2nelist byte0 (map (selN' 0 byte0) (a::l))) :: (valuset2bytesets_rec (map (skipn 1) (a::l)) (i-1)).
+  (list2byteset byte0 (map (selN' 0 byte0) (a::l))) :: (valuset2bytesets_rec (map (skipn 1) (a::l)) (i-1)).
 Proof.
-destruct l; intros; simpl.
-destruct a.
-simpl.
-destruct i.
+destruct i; intros. simpl.
 inversion H.
 simpl.
-rewrite <- minus_n_O; reflexivity.
-simpl.
-destruct i.
-inversion H.
-simpl.
-rewrite <- minus_n_O; reflexivity.
-simpl.
-destruct i.
-inversion H.
-simpl.
-repeat rewrite <- minus_n_O.
+rewrite <- minus_n_O.
 reflexivity.
 Qed.
 
@@ -159,14 +143,7 @@ Proof.
 intros.
 unfold valuset2bytesets.
 apply valuset2bytesets_rec_len.
-unfold nelist2list.
-rewrite map_app.
-unfold not; intros.
-apply length_zero_iff_nil in H.
-rewrite app_length in H.
-simpl in H.
-destruct (length (map valu2list (snd vs))); 
-inversion H.
+unfold not; intros; inversion H.
 Qed.
 
 (* helper le-lt lemmas. *)
@@ -231,7 +208,7 @@ inversion H; reflexivity.
 rewrite H; reflexivity.
 Qed.
 
- (*
+ 
 Lemma concat_hom_selN: forall A (lists: list(list A)) i n k def, 
 Forall (fun sublist => length sublist = k) lists ->
 i < k ->
@@ -269,44 +246,13 @@ remember (n * length a + i) as x.
 replace (length a + n * length a + i) with (length a + x).
 apply le_plus_l.
 omega.
-Qed. *)
+Qed.
 
 
  
-Lemma latest_l2nel: forall A (l:list A) def, 
-  latest(list2nelist def l) =  selN l 0 def.
-Proof.
-induction l; intros.
-reflexivity.
-simpl.
-unfold singular.
-rewrite pushdlist_app.
-rewrite <- minus_n_O.
-destruct (length l).
-reflexivity.
-simpl.
-rewrite rev_unit.
-rewrite rev_involutive.
-rewrite app_nil_r.
-unfold latest.
-reflexivity.
-Qed.
+Lemma fst_list2byteset: forall A (l:list A) def, fst(list2byteset def l) =  selN l 0 def.
+Proof. induction l; intros; reflexivity. Qed.
 
-Lemma selN_make_all_list: forall A (l: list A) i def,
- i < length l ->
-  selN (make_all_list l) i nil = (selN l i def)::nil.
-Proof.
-induction l.
-intros.
-inversion H.
-intros.
-destruct i.
-reflexivity.
-simpl.
-apply IHl.
-simpl in H.
-omega.
-Qed.
 
 Lemma flat_map_len: forall vs, length(flat_map valuset2bytesets vs) = length(vs) * valubytes.
 Proof.
@@ -365,40 +311,77 @@ rewrite H; symmetry; apply plus_n_O.
 unfold not; intros; rewrite H0 in H; inversion H.
 Qed.
 
-Lemma maplatest_mapl2nel: forall A (l: list (list A)) def,
-map (@latest A) (map (list2nelist def) l) = map (selN' 0 def) l.
+Lemma mapfst_maplist2byteset: forall A (l: list (list A)) def,
+map fst (map (list2byteset def) l) = map (selN' 0 def) l.
 Proof.
 intros.
 rewrite map_map.
 unfold selN'.
-replace (fun x : list A => ((list2nelist def) x)!!) with
+replace (fun x : list A => fst (list2byteset def x)) with
   (fun x : list A => selN x 0 def).
 reflexivity.
 apply functional_extensionality.
-intros; symmetry; apply latest_l2nel.
+intros; symmetry; apply fst_list2byteset.
 Qed.
 
 Lemma bcombine_list_contr: forall a l, 
 bcombine (byte2bytes a) (bcombine_list l) = bcombine_list (a::l).
 Proof. intros; reflexivity. Qed.
 
-(* Lemma list2valu2list: forall l, l<>nil -> valu2list (list2valu l) = l.
+Lemma list2valu2list: forall l, l<>nil -> valu2list (list2valu l) = l.
 Proof. Admitted.
 
 Lemma valu2list2valu: forall v, list2valu (valu2list v) = v.
 Proof. Admitted.
- *)
+
 
 
 Lemma cons_simpl: forall A a (l l': list A),
 l = l' -> (a::l) = (a::l').
 Proof. intros; rewrite H; reflexivity. Qed.
 
+Lemma mapfst_v2b_unfold: forall i a vs,
+  i > 0 -> 
+  (map fst (valuset2bytesets_rec (a::vs) i)) = 
+  (selN a 0 byte0):: (map fst (valuset2bytesets_rec (map (skipn 1 )(a::vs)) (i-1))).
+Proof.
+induction i; intros.
+inversion H.
+rewrite valuset2bytesets_rec_expand.
+repeat rewrite map_cons.
+unfold list2byteset.
+replace (S i - 1) with i by omega.
+unfold selN'.
+reflexivity.
+apply H.
+Qed.
+
+
+
+Lemma mapfst_valuset2bytesets: forall i a vs,
+length a = i ->
+(map fst (valuset2bytesets_rec (a::vs) i)) = a.
+Proof.
+induction i; intros.
+apply length_nil in H.
+symmetry; apply H.
+rewrite mapfst_v2b_unfold.
+replace (S i - 1) with i by omega.
+rewrite map_cons.
+rewrite IHi.
+rewrite <- skipn_selN_skipn.
+reflexivity.
+omega.
+rewrite skipn_length.
+omega.
+omega.
+Qed.
+
 Definition cons' {A} (a: list A) b:= cons b a.
 
 Lemma v2b_rec_nil: forall l i,
 i = length l  ->
-valuset2bytesets_rec (l::nil) i = map (list2nelist byte0) (map (cons' nil) l).
+valuset2bytesets_rec (l::nil) i = map (list2byteset byte0) (map (cons' nil) l).
 Proof.
 induction l; intros.
 rewrite H; reflexivity.
@@ -412,36 +395,9 @@ simpl in H.
 inversion H; reflexivity.
 Qed.
 
-Lemma maplatest_v2b: forall  i l,
-  l <> nil ->  length l <= i -> 
-  (map (@latest byte) (valuset2bytesets_rec l i)) = 
-  selN l 0 (byte0::nil).
-Proof. Admitted.
-
-(* Lemma mapfst_valuset2bytesets: forall i a vs,
-length vs >  i ->
-(map (@latest byte) (valuset2bytesets_rec (a::vs) i)) = a.
-Proof.
-induction i; intros.
-simpl.
-apply length_nil in H.
-symmetry; apply H.
-rewrite mapfst_v2b_unfold.
-replace (S i - 1) with i by omega.
-rewrite map_cons.
-rewrite IHi.
-Search cons selN skipn.
-rewrite <- skipn_selN_skipn.
-reflexivity.
-omega.
-rewrite skipn_length.
-omega.
-omega.
-Qed. *)
-
 (* Lemma v2b_rec_selN: forall i j l,
 length l = i -> j < i ->
-selN (valuset2bytesets_rec l i) j byteset0 = list2nelist byteset0 (map (selN' j byte0) l).
+selN (valuset2bytesets_rec l i) j byteset0 = list2byteset byteset0 (map (selN' j byte0) l).
 Proof.
 induction i; intros.
 inversion H0.
@@ -453,7 +409,7 @@ rewrite valuset2bytesets_rec_expand.
 replace (S i - 1) with i by omega.
 rewrite selN_cons.
 rewrite IHi.
-unfold list2nelist.
+unfold list2byteset.
 simpl.
 rewrite map_map.
 simpl.
@@ -465,41 +421,10 @@ simpl.
 simpl.
 destruct j.
 reflexivity.
-unfold list2nelist in IHl.
+unfold list2byteset in IHl.
 destruct a.
 simpl.
 rewrite IHl. *)
-
-(* Lemma skipn_v2b_rec_comm: forall l i j,
-i < j -> length l = j ->
-skipn i (valuset2bytesets_rec l j) = valuset2bytesets_rec (skipn i l) (j-i).
-Proof.
-induction l; intros.
-destruct H0; inversion H.
-
-destruct j. inversion H.
-destruct i.
-rewrite <- minus_n_O.
-reflexivity.
-
-simpl.
-rewrite <- IHl.
-destruct a.
-simpl.
-rewrite valuset2bytesets_rec_expand.
-destruct j.
-inversion H.
-unfold selN'.
-repeat rewrite map_cons.
-rewrite skipn_nil.
-rewrite valuset2bytesets_rec_expand.
-simpl.
-rewrite <- IHl.
-simpl.
-destruct i. reflexivity.
-simpl.
-rewrite <- minus_n_O; reflexivity.
-simpl. *)
 
 
 Lemma bsplit1_bsplit_list: forall sz (b: bytes (1 + (sz - 1))),
@@ -514,7 +439,6 @@ Qed.
 
 Lemma valuset2bytesets2valuset: forall vs, bytesets2valuset (valuset2bytesets vs) = vs.
 Proof. Admitted.
-
 
 Lemma bytesets2valuset2bytesets: forall bs, bs <> nil -> valuset2bytesets (bytesets2valuset bs) = bs.
 Proof. Admitted.
